cfrontend/BeeTypes.v
@@ -164,7 +164,7 @@ match efs with
 | ef' :: efs' => if eq_effect_label ef ef' then true else in_effect ef efs'
 end.
 
-Fixpoint sub_effect (s1 s2 : effect) : bool :=
+Fixpoint sub_effect (s1 s2 : effect) : bool := 
 if s1 is x :: s1' 
 then if s2 is y :: s2' 
      then if eq_effect_label x y 
@@ -496,4 +496,16 @@ sub_effect ef1 ef2 = true ->
 sub_effect ef2 ef3 = true ->
 sub_effect ef1 ef3 = true.
 Proof.
+Admitted.
+
+(* Complete Me: Easy *)
+Lemma prefix_sub_effect : forall (ef1 ef2 : effect), 
+sub_effect ef1 (ef1 ++ ef2)%list = true.
+Proof. 
+Admitted.
+
+(* Complete Me: Easy *)
+Lemma suffix_sub_effect : forall (ef1 ef2 : effect), 
+sub_effect ef2 (ef1 ++ ef2)%list = true.
+Proof. 
 Admitted.
